using the new notation for inline effect annotations in MonotoneSeq

src/tls/MonotoneSeq.fst
@@ -2,50 +2,36 @@ module MonotoneSeq
 open FStar.Seq
 open FStar.SeqProperties
 
-val forall_intro: #a:Type -> #p:(x:a -> GTot Type0) 
-		-> =f:(x:a -> Lemma (p x))
-		-> Lemma (forall (x:a). p x)
-let forall_intro #a #p f = admit()
+let forall_intro (#a:Type) (#p:(x:a -> GTot Type0)) ($f:(x:a -> Lemma (p x)))
+  : Lemma (forall (x:a). p x)
+  = qintro f
 
 (* Some basic stuff, should be moved to FStar.Squash, probably *)
-val forall_intro_2: #a:Type -> #b:(a -> Type) -> #p:(x:a -> b x -> GTot Type0) 
-          -> =f: (x:a -> y:b x -> Lemma (p x y))
-	  -> Lemma (forall (x:a) (y:b x). p x y)
-let forall_intro_2 #a #b #p f = 
-  let g : x:a -> Lemma (forall (y:b x). p x y) = fun x -> forall_intro (f x) in
-  forall_intro g
+let forall_intro_2 (#a:Type) (#b:(a -> Type)) (#p:(x:a -> b x -> GTot Type0))
+                  ($f: (x:a -> y:b x -> Lemma (p x y)))
+  : Lemma (forall (x:a) (y:b x). p x y)
+  = let g : x:a -> Lemma (forall (y:b x). p x y) = fun x -> forall_intro (f x) in
+    forall_intro g
 
-val forall_intro_3: #a:Type -> #b:(a -> Type) -> #c:(x:a -> y:b x -> Type) -> #p:(x:a -> y:b x -> z:c x y -> Type0) 
-          -> =f: (x:a -> y:b x -> z:c x y -> Lemma (p x y z))
-	  -> Lemma (forall (x:a) (y:b x) (z:c x y). p x y z)
-let forall_intro_3 #a #b #c #p f = 
-  let g : x:a -> Lemma (forall (y:b x) (z:c x y). p x y z) = fun x -> forall_intro_2 (f x) in
-  forall_intro g
+let forall_intro_3 (#a:Type) (#b:(a -> Type)) (#c:(x:a -> y:b x -> Type)) (#p:(x:a -> y:b x -> z:c x y -> Type0))
+		  ($f: (x:a -> y:b x -> z:c x y -> Lemma (p x y z)))
+  : Lemma (forall (x:a) (y:b x) (z:c x y). p x y z)
+  = let g : x:a -> Lemma (forall (y:b x) (z:c x y). p x y z) = fun x -> forall_intro_2 (f x) in
+    forall_intro g
 
-val exists_intro: #a:Type -> p:(a -> Type) -> witness:a -> Lemma
-  (requires (p witness))
-  (ensures (exists (x:a). p x))
-let exists_intro (#a:Type) (p:(a -> Type)) witness = ()
+let exists_intro (#a:Type) (p:(a -> Type)) (witness:a)
+  : Lemma (requires (p witness))
+	  (ensures (exists (x:a). p x))
+  = ()
 
-val exists_elim:
-      #a:Type
-    -> #p:(a -> Type)
-    -> #b:Type
-    -> #q:(b -> Type)
-    -> #r:Type
-    -> =f:(x:a -> Lemma (p x ==> r))
-    -> Lemma ((exists (x:a). p x) ==> r)
-let exists_elim #a #p #b #q #r f = forall_intro f
+let exists_elim (#a:Type) (#p:(a -> Type)) (#b:Type) (#q:(b -> Type)) (#r:Type) ($f:(x:a -> Lemma (p x ==> r)))
+  : Lemma ((exists (x:a). p x) ==> r)
+  = forall_intro f
 
-val exists_elim_2: 
-      #a:Type
-    -> #p:(a -> Type)
-    -> #b:Type
-    -> #q:(b -> Type)
-    -> #r:Type
-    -> =f:(x:a -> y:b -> Lemma ((p x /\ q y) ==> r))
-    -> Lemma (((exists (x:a). p x) /\ (exists (y:b). q y)) ==> r)
-let exists_elim_2 #a #p #b #q #r f = forall_intro_2 f
+let exists_elim_2 (#a:Type) (#p:(a -> Type)) (#b:Type) (#q:(b -> Type)) (#r:Type) 
+		 ($f:(x:a -> y:b -> Lemma ((p x /\ q y) ==> r)))
+  : Lemma (((exists (x:a). p x) /\ (exists (y:b). q y)) ==> r)
+  = forall_intro_2 f
 
 ////////////////////////////////////////////////////////////////////////////////
 
@@ -55,131 +41,90 @@ abstract let seq_extension (#a:Type) (s1:seq a) (s2:seq a) (s3:seq a) =
 abstract let grows (#a:Type) (s1:seq a) (s3:seq a) =
   exists (s2:seq a). seq_extension s1 s2 s3
   
-val seq_extension_reflexive: #a:Type -> s:seq a -> Lemma
-  (ensures (grows s s))
-let seq_extension_reflexive #a s =
-  exists_intro (fun w -> seq_extension s w s) (Seq.createEmpty #a)
+let seq_extension_reflexive (#a:Type) (s:seq a) 
+  : Lemma (ensures (grows s s)) 
+  = exists_intro (fun w -> seq_extension s w s) (Seq.createEmpty #a)
 
-val seq_extension_transitive: #a:Type
-  -> s1:seq a
-  -> s2:seq a
-  -> s3:seq a
-  -> s1':seq a
-  -> s2':seq a
-  -> Lemma
-    ((seq_extension s1 s1' s2 
-      /\ seq_extension s2 s2' s3)
-      ==> seq_extension s1 (Seq.append s1' s2') s3)
-let seq_extension_transitive #a s1 s2 s3 s1' s2' = ()
+let seq_extension_transitive (s1:seq 'a) (s2:seq 'a) (s3:seq 'a) (s1':seq 'a) (s2':seq 'a) 
+  : Lemma ((seq_extension s1 s1' s2 /\ seq_extension s2 s2' s3)
+            ==> seq_extension s1 (Seq.append s1' s2') s3) 
+  = ()
 
-val seq_extends_to_transitive_aux: #a:Type
-  -> s1:seq a
-  -> s2:seq a
-  -> s3:seq a
-  -> s1':seq a
-  -> s2':seq a
-  -> Lemma ((seq_extension s1 s1' s2 
-            /\ seq_extension s2 s2' s3)
-          ==> grows s1 s3)
-let seq_extends_to_transitive_aux #a s1 s2 s3 s1' s2' =
-  seq_extension_transitive s1 s2 s3 s1' s2'
+let seq_extends_to_transitive_aux (s1:seq 'a) (s2:seq 'a) (s3:seq 'a) (s1':seq 'a) (s2':seq 'a)
+  : Lemma ((seq_extension s1 s1' s2 /\ seq_extension s2 s2' s3)
+            ==> grows s1 s3) 
+  = seq_extension_transitive s1 s2 s3 s1' s2'
 
+let grows_transitive (s1:seq 'a) (s2:seq 'a) (s3:seq 'a)
+  : Lemma ((grows s1 s2 /\ grows s2 s3)
+           ==> grows s1 s3) 
+  = exists_elim_2 (seq_extends_to_transitive_aux s1 s2 s3)
 
-val grows_transitive: #a:Type
-  -> s1:seq a
-  -> s2:seq a
-  -> s3:seq a
-  -> Lemma ((grows s1 s2 /\ grows s2 s3)
-           ==> grows s1 s3)
-let grows_transitive #a s1 s2 s3 =
-  exists_elim_2 (seq_extends_to_transitive_aux s1 s2 s3)
-
-////////////////////////////////////////////////////////////////////////////////
 open FStar.Monotonic.RRef
 open FStar.HyperHeap
 
-val lemma_grows_monotone: #a:Type
-  -> Lemma (monotonic (seq a) (grows #a))
-let lemma_grows_monotone #a =
-  forall_intro (seq_extension_reflexive #a);
-  forall_intro_3 (grows_transitive #a)
+let lemma_grows_monotone (#a:Type)
+  : Lemma (monotonic (seq a) (grows #a))
+  = forall_intro (seq_extension_reflexive #a);
+    forall_intro_3 (grows_transitive #a)
 
-val snoc : #a:Type -> seq a -> a -> Tot (seq a)
-let snoc #a s x = Seq.append s (Seq.create 1 x)
+let snoc (s:seq 'a) (x:'a) 
+  : Tot (seq 'a) 
+  = Seq.append s (Seq.create 1 x)
 
-val lemma_snoc_extends: #a:Type 
-  -> s:seq a
-  -> x:a 
-  -> Lemma (requires True)
+let lemma_snoc_extends (s:seq 'a) (x:'a)
+  : Lemma (requires True)
 	  (ensures (grows s (snoc s x)))
 	  [SMTPat (grows s (snoc s x))]
-let lemma_snoc_extends #a s x = ()
+  = ()
 
-val lemma_mem_snoc: #a:Type 
-  -> s:seq a
-  -> x:a 
-  -> Lemma 
-    (ensures (SeqProperties.mem x (snoc s x)))
-let lemma_mem_snoc #a s x = SeqProperties.lemma_append_count s (Seq.create 1 x)
+let lemma_mem_snoc (s:seq 'a) (x:'a)
+  : Lemma (ensures (SeqProperties.mem x (snoc s x)))
+  = SeqProperties.lemma_append_count s (Seq.create 1 x)
 
-val alloc_mref_seq: #a:Type -> r:FStar.HyperHeap.rid -> init:seq a
-  -> ST (m_rref r (seq a) grows)
+let alloc_mref_seq (#a:Type) (r:FStar.HyperHeap.rid) (init:seq a)
+  : ST (m_rref r (seq a) grows)
        (requires (fun _ -> True))
        (ensures (fun h0 m h1 -> FStar.ST.ralloc_post r init h0 (as_rref m) h1))
-let alloc_mref_seq #a r init = 
-  lemma_grows_monotone #a;
-  FStar.Monotonic.RRef.m_alloc r init
+  = lemma_grows_monotone #a;
+    FStar.Monotonic.RRef.m_alloc r init
 
+let mem (#a:Type) (#i:rid) (x:a) (r:m_rref i (seq a) grows) (h:t)
+  : GTot Type0
+  = b2t (SeqProperties.mem x (m_sel h r))
 
-(* TODO: this fails with a silly inconsistent qualifier error *)
-(* logic val mem_index: #a:Type -> #i:rid -> n:nat -> x:a -> r:m_rref i (seq a) grows -> t -> GTot Type0 *)
-(* logic let mem_index #a #i n x r h =  *)
-(*       mem x r h *)
-(*       /\ Seq.length (m_sel h r) > n *)
-(*       /\ Seq.index (m_sel h r) n = x *)
-
-val mem : #a:Type -> #i:rid -> x:a -> r:m_rref i (seq a) grows -> t -> GTot Type0
-let mem #a #i x r h = b2t (SeqProperties.mem x (m_sel h r))
-
-let at_least (#a:Type) (#i:rid) (n:nat) (x:a) (r:m_rref i (seq a) grows) (h:t) = 
+let at_least (#a:Type) (#i:rid) (n:nat) (x:a) (r:m_rref i (seq a) grows) (h:t) =
       mem x r h
       /\ Seq.length (m_sel h r) > n
       /\ Seq.index (m_sel h r) n = x
 
-val at_least_is_stable: #a:Type -> #i:rid
-		   -> n:nat
-		   -> x:a
-		   -> r:m_rref i (seq a) grows
-		   -> Lemma (ensures stable_on_t r (at_least n x r))
-let at_least_is_stable #a #i n x r = 
-  let at_least_is_stable_aux: 
+let at_least_is_stable (#a:Type) (#i:rid) (n:nat) (x:a) (r:m_rref i (seq a) grows)
+  : Lemma (ensures stable_on_t r (at_least n x r))
+  = let at_least_is_stable_aux:
 		     h0:t
 		   -> h1:t
 		   -> Lemma ((at_least n x r h0
 			    /\ grows (m_sel h0 r) (m_sel h1 r))
-			    ==> at_least n x r h1) = 
+			    ==> at_least n x r h1) =
        fun h0 h1 -> forall_intro_2 (lemma_mem_append #a) in
-  forall_intro_2 at_least_is_stable_aux
+    forall_intro_2 at_least_is_stable_aux
 
-val write_at_end: #a:Type -> #i:rid
-	       -> r:m_rref i (seq a) grows
-	       -> x:a
-	       -> ST unit
- 		 (requires (fun h -> True))
-		 (ensures (fun h0 _ h1 ->
+let write_at_end (#a:Type) (#i:rid) (r:m_rref i (seq a) grows) (x:a)
+  : ST unit
+       (requires (fun h -> True))
+       (ensures (fun h0 _ h1 ->
 	               m_contains r h1
 		     /\ modifies (Set.singleton i) h0 h1
 		     /\ modifies_rref i !{as_ref (as_rref r)} h0 h1
 		     /\ m_sel h1 r = snoc (m_sel h0 r) x
 		     /\ witnessed (at_least (Seq.length (m_sel h0 r)) x r)))
-let write_at_end #a #i r x =
-  m_recall r;
-  let s0 = m_read r in
-  let n = Seq.length s0 in
-  m_write r (snoc s0 x);
-  at_least_is_stable n x r;
-  lemma_mem_snoc s0 x;
-  witness r (at_least n x r)
+  = m_recall r;
+    let s0 = m_read r in
+    let n = Seq.length s0 in
+    m_write r (snoc s0 x);
+    at_least_is_stable n x r;
+    lemma_mem_snoc s0 x;
+    witness r (at_least n x r)
 
 
 (* An earlier experiment with a weaker witnessed predicate *)
@@ -217,3 +162,11 @@ let write_at_end #a #i r x =
 (* 			    ==> mem x r h1) =  *)
 (*        fun h0 h1 -> forall_intro_2 (lemma_mem_append #a) in *)
 (*   forall_intro_2 mem_is_stable_aux *)
+
+
+(* TODO: this fails with a silly inconsistent qualifier error *)
+(* logic val mem_index: #a:Type -> #i:rid -> n:nat -> x:a -> r:m_rref i (seq a) grows -> t -> GTot Type0 *)
+(* logic let mem_index #a #i n x r h =  *)
+(*       mem x r h *)
+(*       /\ Seq.length (m_sel h r) > n *)
+(*       /\ Seq.index (m_sel h r) n = x *)
